rename Original functions/theorems

Validator/Hedge/Original.lean
@@ -9,7 +9,9 @@ import Validator.Hedge.Denote
 import Validator.Hedge.Grammar
 import Validator.Regex.Regex
 
-theorem decreasing_or_l {α: Type} {σ: Type} [SizeOf σ] (r1 r2: Regex σ) (x: Hedge.Node α):
+namespace Hedge
+
+theorem Grammar.Original.decreasing_or_l {α: Type} {σ: Type} [SizeOf σ] (r1 r2: Regex σ) (x: Hedge.Node α):
   Prod.Lex
     (fun a₁ a₂ => sizeOf a₁ < sizeOf a₂)
     (fun a₁ a₂ => sizeOf a₁ < sizeOf a₂)
@@ -18,7 +20,7 @@ theorem decreasing_or_l {α: Type} {σ: Type} [SizeOf σ] (r1 r2: Regex σ) (x: 
   apply Prod.Lex.right
   simp +arith only [Regex.or.sizeOf_spec]
 
-theorem decreasing_or_r {α: Type} {σ: Type} [SizeOf σ] (r1 r2: Regex σ) (x: Hedge.Node α):
+theorem Grammar.Original.decreasing_or_r {α: Type} {σ: Type} [SizeOf σ] (r1 r2: Regex σ) (x: Hedge.Node α):
   Prod.Lex
     (fun a₁ a₂ => sizeOf a₁ < sizeOf a₂)
     (fun a₁ a₂ => sizeOf a₁ < sizeOf a₂)
@@ -27,7 +29,7 @@ theorem decreasing_or_r {α: Type} {σ: Type} [SizeOf σ] (r1 r2: Regex σ) (x: 
   apply Prod.Lex.right
   simp +arith only [Regex.or.sizeOf_spec]
 
-theorem decreasing_concat_l {α: Type} {σ: Type} [SizeOf σ] (r1 r2: Regex σ) (x: Hedge.Node α):
+theorem Grammar.Original.decreasing_concat_l {α: Type} {σ: Type} [SizeOf σ] (r1 r2: Regex σ) (x: Hedge.Node α):
   Prod.Lex
     (fun a₁ a₂ => sizeOf a₁ < sizeOf a₂)
     (fun a₁ a₂ => sizeOf a₁ < sizeOf a₂)
@@ -36,7 +38,7 @@ theorem decreasing_concat_l {α: Type} {σ: Type} [SizeOf σ] (r1 r2: Regex σ) 
   apply Prod.Lex.right
   simp +arith only [Regex.concat.sizeOf_spec]
 
-theorem decreasing_concat_r {α: Type} {σ: Type} [SizeOf σ] (r1 r2: Regex σ) (x: Hedge.Node α):
+theorem Grammar.Original.decreasing_concat_r {α: Type} {σ: Type} [SizeOf σ] (r1 r2: Regex σ) (x: Hedge.Node α):
   Prod.Lex
     (fun a₁ a₂ => sizeOf a₁ < sizeOf a₂)
     (fun a₁ a₂ => sizeOf a₁ < sizeOf a₂)
@@ -45,7 +47,7 @@ theorem decreasing_concat_r {α: Type} {σ: Type} [SizeOf σ] (r1 r2: Regex σ) 
   apply Prod.Lex.right
   simp +arith only [Regex.concat.sizeOf_spec]
 
-theorem decreasing_star {α: Type} {σ: Type} [SizeOf σ] (r: Regex σ) (x: Hedge.Node α):
+theorem Grammar.Original.decreasing_star {α: Type} {σ: Type} [SizeOf σ] (r: Regex σ) (x: Hedge.Node α):
   Prod.Lex
     (fun a₁ a₂ => sizeOf a₁ < sizeOf a₂)
     (fun a₁ a₂ => sizeOf a₁ < sizeOf a₂)
@@ -54,7 +56,7 @@ theorem decreasing_star {α: Type} {σ: Type} [SizeOf σ] (r: Regex σ) (x: Hedg
   apply Prod.Lex.right
   simp +arith only [Regex.star.sizeOf_spec]
 
-theorem decreasing_symbol {α: Type} {σ: Type} [SizeOf σ] (r1 r2: Regex σ) (label: α) (children: Hedge α) (x: Hedge.Node α) (h: x ∈ children):
+theorem Grammar.Original.decreasing_symbol {α: Type} {σ: Type} [SizeOf σ] (r1 r2: Regex σ) (label: α) (children: Hedge α) (x: Hedge.Node α) (h: x ∈ children):
   Prod.Lex
     (fun a₁ a₂ => sizeOf a₁ < sizeOf a₂)
     (fun a₁ a₂ => sizeOf a₁ < sizeOf a₂)
@@ -65,7 +67,7 @@ theorem decreasing_symbol {α: Type} {σ: Type} [SizeOf σ] (r1 r2: Regex σ) (l
   have h' := List.list_elem_lt h
   omega
 
-theorem decreasing_interleave_l {α: Type} {σ: Type} [SizeOf σ] (r1 r2: Regex σ) (x: Hedge.Node α):
+theorem Grammar.Original.decreasing_interleave_l {α: Type} {σ: Type} [SizeOf σ] (r1 r2: Regex σ) (x: Hedge.Node α):
   Prod.Lex
     (fun a₁ a₂ => sizeOf a₁ < sizeOf a₂)
     (fun a₁ a₂ => sizeOf a₁ < sizeOf a₂)
@@ -74,7 +76,7 @@ theorem decreasing_interleave_l {α: Type} {σ: Type} [SizeOf σ] (r1 r2: Regex 
   apply Prod.Lex.right
   simp +arith only [Regex.interleave.sizeOf_spec]
 
-theorem decreasing_interleave_r {α: Type} {σ: Type} [SizeOf σ] (r1 r2: Regex σ) (x: Hedge.Node α):
+theorem Grammar.Original.decreasing_interleave_r {α: Type} {σ: Type} [SizeOf σ] (r1 r2: Regex σ) (x: Hedge.Node α):
   Prod.Lex
     (fun a₁ a₂ => sizeOf a₁ < sizeOf a₂)
     (fun a₁ a₂ => sizeOf a₁ < sizeOf a₂)
@@ -83,8 +85,8 @@ theorem decreasing_interleave_r {α: Type} {σ: Type} [SizeOf σ] (r1 r2: Regex 
   apply Prod.Lex.right
   simp +arith only [Regex.interleave.sizeOf_spec]
 
-def Original.Rule.derive (G: Hedge.Grammar n φ) (Φ: φ → α → Bool)
-  (r: Regex (φ × Ref n)) (node: Hedge.Node α): Regex (φ × Ref n) :=
+def Grammar.Original.derive (G: Grammar n φ) (Φ: φ → α → Bool)
+  (r: Regex (φ × Ref n)) (node: Node α): Regex (φ × Ref n) :=
   match r with
   | Regex.emptyset => Regex.emptyset
   | Regex.emptystr => Regex.emptyset
@@ -132,14 +134,12 @@ def Original.Rule.derive (G: Hedge.Grammar n φ) (Φ: φ → α → Bool)
 def validate
   (G: Hedge.Grammar n φ) (Φ: φ → α → Bool)
   (r: Regex (φ × Ref n)) (hedge: Hedge α): Bool :=
-  Regex.null (List.foldl (Original.Rule.derive G Φ) r hedge)
+  Regex.null (List.foldl (Grammar.Original.derive G Φ) r hedge)
 
 def run [DecidableEq α] (G: Hedge.Grammar n (AnyEq.Pred α)) (nodes: Hedge α): Bool :=
   validate G AnyEq.Pred.evalb G.start nodes
 
 -- Tests
-
-abbrev node {α} (label: α) children := Hedge.Node.mk label children
 
 #guard run
   (Hedge.Grammar.singleton Regex.emptyset)
@@ -314,9 +314,9 @@ private def example_grammar_sec: Hedge.Grammar 2 String :=
 
 theorem Original.derive_commutes (G: Hedge.Grammar n φ) (Φ: φ → α → Prop)
   [DecidableRel Φ] (r: Regex (φ × Ref n)) (node: Hedge.Node α):
-  Hedge.Grammar.Rule.denote G Φ (Original.Rule.derive G (decideRel Φ) r node)
+  Hedge.Grammar.Rule.denote G Φ (Grammar.Original.derive G (decideRel Φ) r node)
   = Lang.derive (Hedge.Grammar.Rule.denote G Φ r) node := by
-  fun_induction (Rule.derive G (fun p a => Φ p a)) r node with
+  fun_induction (Grammar.Original.derive G (fun p a => Φ p a)) r node with
   | case1 => -- emptyset
     rw [Hedge.Grammar.denote_emptyset]
     rw [Lang.derive_emptyset]
